Isabelle2/Paxos_Sig.thy
@@ -1,0 +1,16 @@
+theory Paxos_Sig
+imports Main Utils IOA
+begin
+
+datatype 'v paxos_action =
+  Propose 'v
+  | Learn inst 'v
+  | Internal
+
+definition paxos_asig where
+"paxos_asig \<equiv>
+  \<lparr> inputs = { Propose c | c . True},
+    outputs = { Learn i v | i v . True},
+    internals = {Internal} \<rparr>"
+
+end
