Isabelle2/Utils.thy
@@ -6,4 +6,7 @@ definition option_as_set where "option_as_set x \<equiv> case x of None \<Righta
   
 abbreviation(input) flip where "flip f \<equiv> \<lambda> x y . f y x"
   
+type_synonym bal = nat
+type_synonym inst = nat
+
 end
